# baseURI: https://w3id.org/nen2660/skos/term
# imports: http://purl.org/dc/elements/1.1/
# imports: http://www.w3.org/2004/02/skos/core

@prefix dcterms: <http://purl.org/dc/terms/> .
@prefix nen2660-term: <https://w3id.org/nen2660/term#> .
@prefix owl: <http://www.w3.org/2002/07/owl#> .
@prefix rdf: <http://www.w3.org/1999/02/22-rdf-syntax-ns#> .
@prefix rdfs: <http://www.w3.org/2000/01/rdf-schema#> .
@prefix skos: <http://www.w3.org/2004/02/skos/core#> .
@prefix xsd: <http://www.w3.org/2001/XMLSchema#> .

<https://w3id.org/nen2660/skos/term>
  a owl:Ontology ;
  a skos:ConceptScheme ;
  owl:imports <http://purl.org/dc/elements/1.1/> ;
  owl:imports <http://www.w3.org/2004/02/skos/core> ;
  skos:hasTopConcept nen2660-term:TopConcept ;
.
nen2660-term:AamountOfBulkMatter
  a skos:Concept ;
  dcterms:issued "2021-06-30T23:59:59.000Z"^^xsd:dateTime ;
  skos:altLabel "batch"@en ;
  skos:altLabel "fluidum"@nl ;
  skos:broader nen2660-term:AamountOfMatter ;
  skos:definition "altDef: reÃ«el object dat bestaat uit een aaneengesloten hoeveelheid niet-vormvaste materie, primair bijeengehouden door externe krachten (zwaartekracht, opsluiting) (bron: NEN 2660-2 (Ontw))"@nl ;
  skos:definition "prefDef: Macroscopisch object, dat bestaat uit een aangesloten hoeveelheid materie zonder vaste structuur (of vaste vorm), en dat primair door externe krachten (zwaartekracht, opsluiting) wordt bijeengehouden. Een hoeveelheid bulkmaterie kan stromen, een discreet object kan bewegen. (bron: Wikipedia, de vrije encyclopedie (NL))"@nl ;
  skos:prefLabel "amount of bulk matter"@en ;
  skos:prefLabel "hoeveelheid bulkmaterie"@nl ;
.
nen2660-term:AamountOfLiquidMatter
  a skos:Concept ;
  dcterms:issued "2021-06-30T23:59:59.000Z"^^xsd:dateTime ;
  skos:broader nen2660-term:AamountOfBulkMatter ;
  skos:definition "prefDef: Bulk materie, bestaand uit een aaneengesloten vloeistofmassa. (bron: Wikipedia, de vrije encyclopedie (NL))"@nl ;
  skos:prefLabel "amount of liquid matter"@en ;
  skos:prefLabel "hoeveelheid vloeibare materie"@nl ;
.
nen2660-term:AamountOfMatter
  a skos:Concept ;
  dcterms:issued "2021-06-30T23:59:59.000Z"^^xsd:dateTime ;
  skos:altLabel "material object, real object"@en ;
  skos:altLabel "materieel object, reeel object"@nl ;
  skos:broader nen2660-term:PhysicalObject ;
  skos:definition "altDef: Physical substance in general, as distinct from mind and spirit (bron: Systems Engineering uitwisselingsstandaard voor de Nederlandse bouwketen (concept))"@en ;
  skos:definition "altDef: fysiek object (vormvast of niet-vormvast) dat tastbaar en zichtbaar is of kan zijn in de werkelijkheid zoals artefacten waaronder bruggen, tanks en apparaten, en  natuurlijke objecten waaronder terreinen, oevers, waterbodems en bomen (bron: NEN 2660-2 (Ontw))"@nl ;
  skos:definition "prefDef: Fysiek object dat bestaat uit een macroscopische hoeveelheid chemische stof, waarvan de afmetingen zodanig zijn dat de klassieke fysica dominant is. Het object kan als een continuum worden behandeld. (bron: Wikipedia, de vrije encyclopedie (NL))"@nl ;
  skos:prefLabel "amount of matter"@en ;
  skos:prefLabel "hoeveelheid materie"@nl ;
.
nen2660-term:AbstractConcept
  a skos:Concept ;
  dcterms:issued "2021-04-15T16:54:00.000Z"^^xsd:dateTime ;
  skos:broader nen2660-term:TopConcept ;
  skos:definition "A representation, objectification or type"@en ;
  skos:prefLabel "Abstract concept"@en ;
.
nen2660-term:Activity
  a skos:Concept ;
  dcterms:issued "2021-04-15T16:54:00.000Z"^^xsd:dateTime ;
  skos:broader nen2660-term:Entity ;
  skos:definition "An activity is something possibly or actually happening in space and time"@en ;
  skos:prefLabel "Activity"@en ;
.
nen2660-term:AggregationStateType
  a skos:Concept ;
  dcterms:issued "2021-04-15T16:54:00.000Z"^^xsd:dateTime ;
  skos:broader nen2660-term:EnumerationType ;
  skos:definition "One of the four fundamental states of matter being solid, liquid, gas or plasma"@en ;
  skos:prefLabel "AggregationStateType"@en ;
.
nen2660-term:AmountOfBulkMatter
  a skos:Concept ;
  dcterms:issued "2021-04-15T16:54:00.000Z"^^xsd:dateTime ;
  skos:broader nen2660-term:RealObject ;
  skos:definition "A real object consisting of a continuous amount of non-rigid (bulk) matter, held together primarily by external forces like gravity or confinement"@en ;
  skos:prefLabel "Amount of bulk matter"@en ;
.
nen2660-term:ChemicalBonding
  a skos:Concept ;
  dcterms:issued "2021-04-15T16:54:00.000Z"^^xsd:dateTime ;
  skos:broader nen2660-term:PureSubstance ;
  skos:definition "Pure substance consisting of two or more chemical elements that have a chemical bond with each other. In a chemical bonding, the elements occur in a fixed ratio. A compound can be broken down into simpler substances by means of chemical reactions"@en ;
  skos:prefLabel "Chemical bonding"@en ;
.
nen2660-term:ChemicalElement
  a skos:Concept ;
  dcterms:issued "2021-04-15T16:54:00.000Z"^^xsd:dateTime ;
  skos:broader nen2660-term:PureSubstance ;
  skos:definition "Pure substance that is made up of atoms with the same atomic number. A chemical element cannot be decomposed through chemical reactions"@en ;
  skos:prefLabel "Chemical element"@en ;
.
nen2660-term:Client
  a skos:Concept ;
  dcterms:issued "2021-04-15T16:54:00.000Z"^^xsd:dateTime ;
  skos:broader nen2660-term:RequirementSourceType ;
  skos:definition "A customer, a buyer or receiver of goods or services"@en ;
  skos:prefLabel "Client"@en ;
.
nen2660-term:ComputationalObject
  a skos:Concept ;
  dcterms:issued "2021-04-15T16:54:00.000Z"^^xsd:dateTime ;
  skos:broader nen2660-term:InformationObject ;
  skos:definition "prefDef: Object, dat bestaat of kan bestaan binnen de runtime omgeving van een computer. (bron: NEN 2660-1 (Ontw))"@nl ;
  skos:prefLabel "computational object"@en ;
  skos:prefLabel "rekenkundig object"@nl ;
.
nen2660-term:ConcreteConcept
  a skos:Concept ;
  dcterms:issued "2021-04-15T16:54:00.000Z"^^xsd:dateTime ;
  skos:broader nen2660-term:TopConcept ;
  skos:definition "An entity, event or state"@en ;
  skos:prefLabel "Concrete concept"@en ;
.
nen2660-term:Connection
  a skos:Concept ;
  dcterms:issued "2021-04-15T16:54:00.000Z"^^xsd:dateTime ;
  skos:broader nen2660-term:PhysicalObject ;
  skos:definition "The thing at which two or more things are connected"@en ;
  skos:prefLabel "Connection"@en ;
.
nen2660-term:Definition
  a skos:Concept ;
  dcterms:issued "2021-04-15T16:54:00.000Z"^^xsd:dateTime ;
  skos:broader nen2660-term:RequirementSourceType ;
  skos:definition "A statement of the meaning of a word or word group or a sign or symbol"@en ;
  skos:prefLabel "Definition"@en ;
.
nen2660-term:Demand
  a skos:Concept ;
  dcterms:issued "2021-04-15T16:54:00.000Z"^^xsd:dateTime ;
  skos:broader nen2660-term:RequirementSeverityType ;
  skos:definition "An urgent request or forceful claim"@en ;
  skos:prefLabel "Demand"@en ;
.
nen2660-term:DiscreteObject
  a skos:Concept ;
  dcterms:issued "2021-04-15T16:54:00.000Z"^^xsd:dateTime ;
  skos:broader nen2660-term:RealObject ;
  skos:definition "A real object consisting of a contiguous amount of form-retaining matter, held together primarily by internal forces (gravity, electromagnetic force)"@en ;
  skos:prefLabel "Discrete object"@en ;
.
nen2660-term:EnergyFlow
  a skos:Concept ;
  dcterms:issued "2021-04-15T16:54:00.000Z"^^xsd:dateTime ;
  skos:broader nen2660-term:TransferType ;
  skos:definition "The movement of an amount of energy (as capacity to do work)"@en ;
  skos:prefLabel "Energy flow"@en ;
.
nen2660-term:Entity
  a skos:Concept ;
  dcterms:issued "2021-04-15T16:54:00.000Z"^^xsd:dateTime ;
  skos:broader nen2660-term:ConcreteConcept ;
  skos:definition "An object or an activity"@en ;
  skos:prefLabel "Entity"@en ;
.
nen2660-term:EnumerationType
  a skos:Concept ;
  dcterms:issued "2021-04-15T16:54:00.000Z"^^xsd:dateTime ;
  skos:broader nen2660-term:Type ;
  skos:definition "A type having a fixed or extendable set of simple instances having no further attributes or relations"@en ;
  skos:prefLabel "EnumerationType"@en ;
.
nen2660-term:Event
  a skos:Concept ;
  dcterms:issued "2021-04-15T16:54:00.000Z"^^xsd:dateTime ;
  skos:broader nen2660-term:ConcreteConcept ;
  skos:definition "A thing that happens or takes place and marks the beginning or ending of a state"@en ;
  skos:prefLabel "Event"@en ;
.
nen2660-term:Fluid
  a skos:Concept ;
  dcterms:issued "2021-04-15T16:54:00.000Z"^^xsd:dateTime ;
  skos:broader nen2660-term:AggregationStateType ;
  skos:definition "One of the four fundamental states of matter"@en ;
  skos:prefLabel "Fluid"@en ;
.
nen2660-term:Force
  a skos:Concept ;
  dcterms:issued "2021-04-15T16:54:00.000Z"^^xsd:dateTime ;
  skos:broader nen2660-term:TransferType ;
  skos:definition "A physical quantity that denotes ability to push, pull, twist or accelerate a body"@en ;
  skos:prefLabel "Force"@en ;
.
nen2660-term:FunctionalEntity
  a skos:Concept ;
  dcterms:issued "2021-04-15T16:54:00.000Z"^^xsd:dateTime ;
  skos:broader nen2660-term:Entity ;
  skos:definition "An entity involving the external behavior (function) of the object where the output contributes to stakeholder objectives (what it does) implemented/played by a technical entities"@en ;
  skos:prefLabel "Functional entity"@en ;
.
nen2660-term:Gas
  a skos:Concept ;
  dcterms:issued "2021-04-15T16:54:00.000Z"^^xsd:dateTime ;
  skos:broader nen2660-term:AggregationStateType ;
  skos:definition "Matter in an intermediate state between liquid and plasma that can be contained only if it is fully surrounded by a solid (or in a bubble of liquid) (or held together by gravitational pull); it can condense into a liquid, or can (rarely) become a solid directly by deposition"@en ;
  skos:prefLabel "Gas"@en ;
.
nen2660-term:GeometricEntity
  a skos:Concept ;
  dcterms:issued "2021-04-15T16:54:00.000Z"^^xsd:dateTime ;
  skos:broader nen2660-term:Representation ;
  skos:definition "A spatial representation"@en ;
  skos:prefLabel "GeometricEntity"@en ;
.
nen2660-term:HeterogeneousMixture
  a skos:Concept ;
  dcterms:issued "2021-04-15T16:54:00.000Z"^^xsd:dateTime ;
  skos:broader nen2660-term:Mixture ;
  skos:definition "A mixture that is separated into different regions or phases that have different compositions or properties"@en ;
  skos:prefLabel "Heterogeneous mixture"@en ;
.
nen2660-term:HomogeneousMixture
  a skos:Concept ;
  dcterms:issued "2021-04-15T16:54:00.000Z"^^xsd:dateTime ;
  skos:broader nen2660-term:Mixture ;
  skos:definition "A mixture that is uniform throughout, and has only one phase"@en ;
  skos:prefLabel "Homogeneous mixture"@en ;
.
nen2660-term:InformationFlow
  a skos:Concept ;
  dcterms:issued "2021-04-15T16:54:00.000Z"^^xsd:dateTime ;
  skos:broader nen2660-term:TransferType ;
  skos:definition "The movement of information represented in some medium"@en ;
  skos:prefLabel "Information flow"@en ;
.
nen2660-term:InformationObject
  a skos:Concept ;
  dcterms:issued "2021-04-15T16:54:00.000Z"^^xsd:dateTime ;
  skos:broader nen2660-term:Object ;
  skos:definition "Thing that is a whole of information on itself and has an own identity"@en ;
  skos:prefLabel "Information object"@en ;
.
nen2660-term:Interaction
  a skos:Concept ;
  dcterms:issued "2021-04-15T16:54:00.000Z"^^xsd:dateTime ;
  skos:broader nen2660-term:Activity ;
  skos:definition "The activity in which two or more objects act upon one another to produce a new effect"@en ;
  skos:prefLabel "Interaction"@en ;
.
nen2660-term:Interface
  a skos:Concept ;
  dcterms:issued "2021-04-15T16:54:00.000Z"^^xsd:dateTime ;
  skos:broader nen2660-term:SpatialRegion ;
  skos:definition "The spatial region being a point of interaction between entities"@en ;
  skos:prefLabel "Interface"@en ;
.
nen2660-term:LawOrRegulation
  a skos:Concept ;
  dcterms:issued "2021-04-15T16:54:00.000Z"^^xsd:dateTime ;
  skos:broader nen2660-term:RequirementSourceType ;
  skos:definition "The body of binding rules and regulations, customs and standards established in a community by its legislative and judicial authorities"@en ;
  skos:prefLabel "Law or regulation"@en ;
.
nen2660-term:MaterialFlow
  a skos:Concept ;
  dcterms:issued "2021-04-15T16:54:00.000Z"^^xsd:dateTime ;
  skos:broader nen2660-term:TransferType ;
  skos:definition "The movement of an amount of matter"@en ;
  skos:prefLabel "Material flow"@en ;
.
nen2660-term:Matter
  a skos:Concept ;
  dcterms:issued "2021-04-15T16:54:00.000Z"^^xsd:dateTime ;
  skos:altLabel "Chemical substance"@en ;
  skos:broader nen2660-term:PhysicalObject ;
  skos:definition "A pure chemical substance, chemical bonding or mixture from which real objects are made"@en ;
  skos:prefLabel "Matter"@en ;
.
nen2660-term:MatterPortion
  a skos:Concept ;
  dcterms:issued "2021-04-15T16:54:00.000Z"^^xsd:dateTime ;
  skos:broader nen2660-term:RelationReference ;
  skos:definition "An objectified relation reference for the 'consists of' relation"@en ;
  skos:prefLabel "MatterPortion"@en ;
.
nen2660-term:Mixture
  a skos:Concept ;
  dcterms:issued "2021-04-15T16:54:00.000Z"^^xsd:dateTime ;
  skos:broader nen2660-term:Matter ;
  skos:definition "Matter that consists of multiple forms of pure matter"@en ;
  skos:prefLabel "Mixture"@en ;
.
nen2660-term:Object
  a skos:Concept ;
  dcterms:issued "2021-04-15T16:54:00.000Z"^^xsd:dateTime ;
  skos:broader nen2660-term:Entity ;
  skos:definition "A physical object or an information object"@en ;
  skos:prefLabel "Object"@en ;
.
nen2660-term:ObjectType
  a skos:Concept ;
  dcterms:issued "2021-04-15T16:54:00.000Z"^^xsd:dateTime ;
  skos:broader nen2660-term:Type ;
  skos:definition "A type having a fixed or extendable set of instances that can have attributes or relations of its own"@en ;
  skos:prefLabel "ObjectType"@en ;
.
nen2660-term:Objectification
  a skos:Concept ;
  dcterms:issued "2021-04-15T16:54:00.000Z"^^xsd:dateTime ;
  skos:broader nen2660-term:AbstractConcept ;
  skos:definition "An attribute (quality or quantity) or relation represented as an individual defined by a concept"@en ;
  skos:prefLabel "Objectification"@en ;
.
nen2660-term:PhysicalObject
  a skos:Concept ;
  dcterms:issued "2021-04-15T16:54:00.000Z"^^xsd:dateTime ;
  skos:broader nen2660-term:Object ;
  skos:definition "Something that possibly or actually exists in space and time, perceivable through the senses"@en ;
  skos:prefLabel "Physical object"@en ;
.
nen2660-term:PlannedEntity
  a skos:Concept ;
  dcterms:issued "2021-04-15T16:54:00.000Z"^^xsd:dateTime ;
  skos:broader nen2660-term:Entity ;
  skos:definition "An entity that does not yet exist or does not yet exist in the desired form"@en ;
  skos:prefLabel "Planned entity"@en ;
.
nen2660-term:Plasma
  a skos:Concept ;
  dcterms:issued "2021-04-15T16:54:00.000Z"^^xsd:dateTime ;
  skos:broader nen2660-term:AggregationStateType ;
  skos:definition "One of the four fundamental states of matter"@en ;
  skos:prefLabel "Plasma"@en ;
.
nen2660-term:Port
  a skos:Concept ;
  dcterms:issued "2021-04-15T16:54:00.000Z"^^xsd:dateTime ;
  skos:broader nen2660-term:PhysicalObject ;
  skos:definition "Explicit part of an entity where interaction with other entities can take place via a connection or interface"@en ;
  skos:prefLabel "Port"@en ;
.
nen2660-term:PureSubstance
  a skos:Concept ;
  dcterms:issued "2021-04-15T16:54:00.000Z"^^xsd:dateTime ;
  skos:broader nen2660-term:Matter ;
  skos:definition "Matter that has an equal chemical composition and recognizable uniform and isotropic properties"@en ;
  skos:prefLabel "Pure substance"@en ;
.
nen2660-term:QualityValue
  a skos:Concept ;
  dcterms:issued "2021-04-15T16:54:00.000Z"^^xsd:dateTime ;
  skos:broader nen2660-term:Objectification ;
  skos:definition "The objectification of a value of a quality having a complex value like a simple value sec combined with other metadata or just a combination of simple values"@en ;
  skos:prefLabel "QualityValue"@en ;
.
nen2660-term:QuantityKind
  a skos:Concept ;
  dcterms:issued "2021-04-15T16:54:00.000Z"^^xsd:dateTime ;
  skos:definition "Base or derived kind of quantity like length or time"@en ;
  skos:prefLabel "QuantityKind"@en ;
.
nen2660-term:QuantityValue
  a skos:Concept ;
  dcterms:issued "2021-04-15T16:54:00.000Z"^^xsd:dateTime ;
  skos:broader nen2660-term:Objectification ;
  skos:definition "The objectification of a value of a quantity (involving a quantitykind and a unit) having a complex value like a simple value sec combined with other metadata or just a combination of simple values"@en ;
  skos:prefLabel "QuantityValue"@en ;
.
nen2660-term:RealObject
  a skos:Concept ;
  dcterms:issued "2021-04-15T16:54:00.000Z"^^xsd:dateTime ;
  skos:altLabel "Amount of matter"@en ;
  skos:broader nen2660-term:PhysicalObject ;
  skos:definition "A physical object that can be tangible and visible in reality such as artifacts including bridges, tanks and devices, and natural objects including terrains, banks, water bottoms and trees"@en ;
  skos:prefLabel "Real object"@en ;
.
nen2660-term:RealizedEntity
  a skos:Concept ;
  dcterms:issued "2021-04-15T16:54:00.000Z"^^xsd:dateTime ;
  skos:broader nen2660-term:Entity ;
  skos:definition "An entity that exists or has existed"@en ;
  skos:prefLabel "Realized entity"@en ;
.
nen2660-term:RelationReference
  a skos:Concept ;
  dcterms:issued "2021-04-15T16:54:00.000Z"^^xsd:dateTime ;
  skos:broader nen2660-term:Objectification ;
  skos:definition "The objectification of a reference for a relation having a complex value like a simple reference sec combined with other metadata or just a combination of simple references (n-ary relationships)"@en ;
  skos:prefLabel "RelationReference"@en ;
.
nen2660-term:Representation
  a skos:Concept ;
  dcterms:issued "2021-04-15T16:54:00.000Z"^^xsd:dateTime ;
  skos:broader nen2660-term:AbstractConcept ;
  skos:definition "That which represents something else"@en ;
  skos:prefLabel "Representation"@en ;
.
nen2660-term:Requirement
  a skos:Concept ;
  dcterms:issued "2021-04-15T16:54:00.000Z"^^xsd:dateTime ;
  skos:broader nen2660-term:InformationObject ;
  skos:definition "A rule that should hold for something, defined w.r.t. to its attributes or relations" ;
  skos:prefLabel "Requirement"@en ;
.
nen2660-term:RequirementSeverityType
  a skos:Concept ;
  dcterms:issued "2021-04-15T16:54:00.000Z"^^xsd:dateTime ;
  skos:broader nen2660-term:EnumerationType ;
  skos:definition "The serieusness of a requirement, here: demand or wish"@en ;
  skos:prefLabel "RequirementSeverityType"@en ;
.
nen2660-term:RequirementSourceType
  a skos:Concept ;
  dcterms:issued "2021-04-15T16:54:00.000Z"^^xsd:dateTime ;
  skos:broader nen2660-term:EnumerationType ;
  skos:definition "The person, organization, place or thing from which a requirement comes, here: a client, definition, sector or law/regulation"@en ;
  skos:prefLabel "RequirementSourceType"@en ;
.
nen2660-term:Sector
  a skos:Concept ;
  dcterms:issued "2021-04-15T16:54:00.000Z"^^xsd:dateTime ;
  skos:broader nen2660-term:RequirementSourceType ;
  skos:definition "A public or private field of economic activity"@en ;
  skos:prefLabel "Sector"@en ;
.
nen2660-term:Solid
  a skos:Concept ;
  dcterms:issued "2021-04-15T16:54:00.000Z"^^xsd:dateTime ;
  skos:broader nen2660-term:AggregationStateType ;
  skos:definition "Matter that can be picked up or held, having a texture, and usually firm. Unlike a liquid, gas or plasma"@en ;
  skos:prefLabel "Solid"@en ;
.
nen2660-term:SpatialRegion
  a skos:Concept ;
  dcterms:issued "2021-04-15T16:54:00.000Z"^^xsd:dateTime ;
  skos:broader nen2660-term:PhysicalObject ;
  skos:definition "A physical object that encloses a certain area such as rooms, roads and rivers that is bound by real objects, other spacetial regions or based on use or convention and that is empty or contains discrete or liquid or gaseous matter"@en ;
  skos:prefLabel "Spatial region"@en ;
.
nen2660-term:State
  a skos:Concept ;
  dcterms:issued "2021-04-15T16:54:00.000Z"^^xsd:dateTime ;
  skos:broader nen2660-term:ConcreteConcept ;
  skos:definition "A temporal part of an entity during a period between events. A state is characterized by the attributes and relationships of the entity. â"@en ;
  skos:prefLabel "State"@en ;
.
nen2660-term:SymbolicObject
  a skos:Concept ;
  dcterms:issued "2021-04-15T16:54:00.000Z"^^xsd:dateTime ;
  skos:broader nen2660-term:InformationObject ;
  skos:definition "prefDef: Object dat wordt uitgewisseld, of kan worden uitgewisseld,  tijdens communicatie tussen twee of meer actoren (sociale actoren of computer actoren). Een symbolisch object is een drager van informatie, en wordt op zijn beurt gedragen door een fysiek object. Een symbolisch object wordt uitgedrukt in een taal. (bron: NEN 2660-1 (Ontw))"@nl ;
  skos:prefLabel "symbolic object"@en ;
  skos:prefLabel "symbolisch object"@nl ;
.
nen2660-term:TechnicalEntity
  a skos:Concept ;
  dcterms:issued "2021-04-15T16:54:00.000Z"^^xsd:dateTime ;
  skos:broader nen2660-term:Entity ;
  skos:definition "An entity having technical properties and relations (what it is) that implements/plays functional entities"@en ;
  skos:prefLabel "Technical object"@en ;
.
nen2660-term:TemporalEntity
  a skos:Concept ;
  dcterms:issued "2021-04-15T16:54:00.000Z"^^xsd:dateTime ;
  skos:broader nen2660-term:Representation ;
  skos:definition "A temporal representation"@en ;
  skos:prefLabel "TemporalEntity"@en ;
.
nen2660-term:Thought
  a skos:Concept ;
  dcterms:issued "2021-04-15T16:54:00.000Z"^^xsd:dateTime ;
  skos:broader nen2660-term:InformationObject ;
  skos:definition "prefDef: Object, dat bestaat of kan bestaan in de gedachte van een persoon. (bron: NEN 2660-1 (Ontw))"@nl ;
  skos:prefLabel "mentaal object"@nl ;
  skos:prefLabel "thought"@en ;
.
nen2660-term:TopConcept
  a skos:Concept ;
  dcterms:issued "2021-04-15T16:54:00.000Z"^^xsd:dateTime ;
  skos:definition "The most generic root concept of nen2660"@en ;
  skos:prefLabel "Top concept"@en ;
.
nen2660-term:TransferType
  a skos:Concept ;
  dcterms:issued "2021-04-15T16:54:00.000Z"^^xsd:dateTime ;
  skos:broader nen2660-term:EnumerationType ;
  skos:definition "The type of thing being transferred, here: material, information, energy or force"@en ;
  skos:prefLabel "TransferType"@en ;
.
nen2660-term:Type
  a skos:Concept ;
  dcterms:issued "2021-04-15T16:54:00.000Z"^^xsd:dateTime ;
  skos:broader nen2660-term:AbstractConcept ;
  skos:definition "A meta-concept which instances are concepts (not individuals)"@en ;
  skos:prefLabel "Type"@en ;
.
nen2660-term:Unit
  a skos:Concept ;
  dcterms:issued "2021-04-15T16:54:00.000Z"^^xsd:dateTime ;
  skos:definition "A scale of measurement"@en ;
  skos:prefLabel "Unit"@en ;
.
nen2660-term:Wish
  a skos:Concept ;
  dcterms:issued "2021-04-15T16:54:00.000Z"^^xsd:dateTime ;
  skos:broader nen2660-term:RequirementSeverityType ;
  skos:definition "A 'nice to have' requirement"@en ;
  skos:prefLabel "Wish"@en ;
.
nen2660-term:abbreviation
  a skos:Concept ;
  dcterms:issued "2021-04-15T16:54:00.000Z"^^xsd:dateTime ;
  skos:broader skos:altLabel ;
  skos:definition "Acronym or initial word as special case of an external name"@en ;
  skos:prefLabel "abbreviation"@en ;
.
nen2660-term:aggregationStateType
  a skos:Concept ;
  dcterms:issued "2021-04-15T16:54:00.000Z"^^xsd:dateTime ;
  skos:definition "The possession of an aggregation state type"@en ;
  skos:prefLabel "aggregation state type"@en ;
.
nen2660-term:amountOfIndividuals
  a skos:Concept ;
  dcterms:issued "2021-04-15T16:54:00.000Z"^^xsd:dateTime ;
  skos:definition "The possession of an amount of individuals by a container modelling an implicit group"@en ;
  skos:prefLabel "amount of individuals"@en ;
.
nen2660-term:begins
  a skos:Concept ;
  dcterms:issued "2021-04-15T16:54:00.000Z"^^xsd:dateTime ;
  skos:definition "The state that is started by an event"@en ;
  skos:prefLabel "begins"@en ;
.
nen2660-term:chemicalFormula
  a skos:Concept ;
  dcterms:issued "2021-04-15T16:54:00.000Z"^^xsd:dateTime ;
  skos:definition "The possession of information about the chemical proportions of atoms that constitute a particular chemical bonding"@en ;
  skos:prefLabel "chemical formula"@en ;
.
nen2660-term:connectsObject
  a skos:Concept ;
  dcterms:issued "2021-04-15T16:54:00.000Z"^^xsd:dateTime ;
  skos:definition "The physical objects connected by a connection or interface"@en ;
  skos:prefLabel "connects object"@en ;
.
nen2660-term:connectsPort
  a skos:Concept ;
  dcterms:issued "2021-04-15T16:54:00.000Z"^^xsd:dateTime ;
  skos:definition "The ports (as part of physical objects) connected by a connection or interface"@en ;
  skos:prefLabel "connects port"@en ;
.
nen2660-term:consistsOf
  a skos:Concept ;
  dcterms:issued "2021-04-15T16:54:00.000Z"^^xsd:dateTime ;
  skos:definition "The matter a real object, mixture or matter portion is made of"@en ;
  skos:prefLabel "consists of"@en ;
.
nen2660-term:ends
  a skos:Concept ;
  dcterms:issued "2021-04-15T16:54:00.000Z"^^xsd:dateTime ;
  skos:definition "The state that is ended by an event"@en ;
  skos:prefLabel "ends"@en ;
.
nen2660-term:hasBoundary
  a skos:Concept ;
  dcterms:issued "2021-04-15T16:54:00.000Z"^^xsd:dateTime ;
  skos:definition "The geometric entity representing the boundary of a concrete concept"@en ;
  skos:prefLabel "has boundary"@en ;
.
nen2660-term:hasFunctionalPart
  a skos:Concept ;
  dcterms:issued "2021-04-15T16:54:00.000Z"^^xsd:dateTime ;
  skos:broader nen2660-term:hasPart ;
  skos:definition "The hasPart relation of a functional nature"@en ;
  skos:prefLabel "has functional part"@en ;
.
nen2660-term:hasInterior
  a skos:Concept ;
  dcterms:issued "2021-04-15T16:54:00.000Z"^^xsd:dateTime ;
  skos:definition "The geometric entity representing the interior of a concrete concept"@en ;
  skos:prefLabel "has interior"@en ;
.
nen2660-term:hasPart
  a skos:Concept ;
  dcterms:issued "2021-04-15T16:54:00.000Z"^^xsd:dateTime ;
  skos:definition "A decomposition relationship between physical objects themselves, between information objects themselves or between activities themselves"@en ;
  skos:prefLabel "has part"@en ;
.
nen2660-term:hasQuantityKind
  a skos:Concept ;
  dcterms:issued "2021-04-15T16:54:00.000Z"^^xsd:dateTime ;
  skos:definition "The possession of a quantity kind as defined by QUDT"@en ;
  skos:prefLabel "has quantity kind"@en ;
.
nen2660-term:hasRequirement
  a skos:Concept ;
  dcterms:issued "2021-04-15T16:54:00.000Z"^^xsd:dateTime ;
  skos:definition "The (unstructured) requirement for something"@en ;
  skos:prefLabel "has requirement"@en ;
.
nen2660-term:hasRequirementSpecification
  a skos:Concept ;
  dcterms:issued "2021-04-15T16:54:00.000Z"^^xsd:dateTime ;
  skos:definition "The possession of a requirement specification by a requirement"@en ;
  skos:prefLabel "has requirement specification"@en ;
.
nen2660-term:hasState
  a skos:Concept ;
  dcterms:issued "2021-04-15T16:54:00.000Z"^^xsd:dateTime ;
  skos:definition "The state of an entity in a certain point or period of time"@en ;
  skos:prefLabel "has state"@en ;
.
nen2660-term:hasTechnicalPart
  a skos:Concept ;
  dcterms:issued "2021-04-15T16:54:00.000Z"^^xsd:dateTime ;
  skos:broader nen2660-term:hasPart ;
  skos:definition "A hasPart relation of a technical nature"@en ;
  skos:prefLabel "has technical part"@en ;
.
nen2660-term:hasTemporalEntity
  a skos:Concept ;
  dcterms:issued "2021-04-15T16:54:00.000Z"^^xsd:dateTime ;
  skos:definition "The temporal entity representing a concrete concept in time"@en ;
  skos:prefLabel "has temporal entity"@en ;
.
nen2660-term:hasUnit
  a skos:Concept ;
  dcterms:issued "2021-04-15T16:54:00.000Z"^^xsd:dateTime ;
  skos:definition "The possession of a unit as defined by QUDT"@en ;
  skos:prefLabel "has unit"@en ;
.
nen2660-term:isBoundBy
  a skos:Concept ;
  dcterms:issued "2021-04-15T16:54:00.000Z"^^xsd:dateTime ;
  skos:definition "The physical object that bounds a spatial region"@en ;
  skos:prefLabel "is bound by"@en ;
.
nen2660-term:isConnectedTo
  a skos:Concept ;
  dcterms:issued "2021-04-15T16:54:00.000Z"^^xsd:dateTime ;
  skos:definition "The topological relationship between physical objects"@en ;
  skos:prefLabel "is connected to"@en ;
.
nen2660-term:isDescribedBy
  a skos:Concept ;
  dcterms:issued "2021-04-15T16:54:00.000Z"^^xsd:dateTime ;
  skos:definition "The information object that describes something"@en ;
  skos:prefLabel "is described by"@en ;
.
nen2660-term:isImplementedBy
  a skos:Concept ;
  dcterms:issued "2021-04-15T16:54:00.000Z"^^xsd:dateTime ;
  skos:definition "The technical entity that implements a functional entity"@en ;
  skos:prefLabel "is implemented by"@en ;
.
nen2660-term:isRealizedBy
  a skos:Concept ;
  dcterms:issued "2021-04-15T16:54:00.000Z"^^xsd:dateTime ;
  skos:definition "The realized entity that realizes a planned entity"@en ;
  skos:prefLabel "is realized by"@en ;
.
nen2660-term:overConnection
  a skos:Concept ;
  dcterms:issued "2021-04-15T16:54:00.000Z"^^xsd:dateTime ;
  skos:definition "The connection over which an interaction between physical objects takes place"@en ;
  skos:prefLabel "over connection"@en ;
.
nen2660-term:overInterface
  a skos:Concept ;
  dcterms:issued "2021-04-15T16:54:00.000Z"^^xsd:dateTime ;
  skos:definition "The interface over which an interaction between physical objects takes place"@en ;
  skos:prefLabel "over interface"@en ;
.
nen2660-term:participatesIn
  a skos:Concept ;
  dcterms:issued "2021-04-15T16:54:00.000Z"^^xsd:dateTime ;
  skos:definition "The interaction a physical object participates in"@en ;
  skos:prefLabel "participates in"@en ;
.
nen2660-term:performs
  a skos:Concept ;
  dcterms:issued "2021-04-15T16:54:00.000Z"^^xsd:dateTime ;
  skos:definition "The activity performed by a physical object"@en ;
  skos:prefLabel "performs"@en ;
.
nen2660-term:portion
  a skos:Concept ;
  dcterms:issued "2021-04-15T16:54:00.000Z"^^xsd:dateTime ;
  skos:definition "The actual relative portion of a matter portion"@en ;
  skos:prefLabel "portion"@en ;
.
nen2660-term:requirementSeverityType
  a skos:Concept ;
  dcterms:issued "2021-04-15T16:54:00.000Z"^^xsd:dateTime ;
  skos:definition "The possession of a severity type by a requirement"@en ;
  skos:prefLabel "requirement severity type"@en ;
.
nen2660-term:requirementSourceType
  a skos:Concept ;
  dcterms:issued "2021-04-15T16:54:00.000Z"^^xsd:dateTime ;
  skos:definition "The possession of a source type by a requirement"@en ;
  skos:prefLabel "requirement source type"@en ;
.
nen2660-term:transferType
  a skos:Concept ;
  dcterms:issued "2021-04-15T16:54:00.000Z"^^xsd:dateTime ;
  skos:definition "The possession of a transfer type by an interaction"@en ;
  skos:prefLabel "transfer type"@en ;
.
nen2660-term:transforms
  a skos:Concept ;
  dcterms:issued "2021-04-15T16:54:00.000Z"^^xsd:dateTime ;
  skos:definition "The object transformed by an activity"@en ;
  skos:prefLabel "transforms"@en ;
.
nen2660-term:triggers
  a skos:Concept ;
  dcterms:issued "2021-04-15T16:54:00.000Z"^^xsd:dateTime ;
  skos:definition "The event triggert by an entity"@en ;
  skos:prefLabel "triggers"@en ;
.
nen2660-term:typeOfIndividuals
  a skos:Concept ;
  dcterms:issued "2021-04-15T16:54:00.000Z"^^xsd:dateTime ;
  skos:definition "The possession of a type of individuals by a container modelling an implicit group"@en ;
  skos:prefLabel "type of individuals"@en ;
.
